CslibTests.lean
@@ -13,5 +13,6 @@ public import CslibTests.ImportWithMathlib
 public import CslibTests.LTS
 public import CslibTests.LambdaCalculus
 public import CslibTests.MLL
+public import CslibTests.ModalFrameSeparation
 public import CslibTests.Propositional
 public import CslibTests.Reduction
